Strata/DL/Lambda/Semantics.lean
@@ -11,7 +11,7 @@ import Strata.DL.Lambda.LState
 
 ---------------------------------------------------------------------
 
-namespace Lamda
+namespace Lambda
 
 variable {IDMeta:Type} [DecidableEq IDMeta]
 
@@ -21,80 +21,76 @@ open Lambda
 A small-step semantics of LExpr.
 Currently only defined for LMonoTy, but it will be expanded to an arbitrary
 type.
+The order of constructors matter because the `constructor` tactic will rely on
+it.
+This small-step definitions faithfully follows the behavior of LExpr.eval,
+except that this inductive definition may stuck early when there is no
+assignment to a free variable available in LState.
 -/
 inductive Step
   : LState IDMeta → LExpr LMonoTy IDMeta → LExpr LMonoTy IDMeta → Prop where
--- A small-step reduction expands functions and free variables when they are
--- evaluated. Stucks if the function body is unknown or fvar does not exist
--- in LState.
-| expand_fn:
-  ∀ (σ:LState IDMeta) (func_id:Identifier IDMeta) (fn:LFunc IDMeta)
-    (fnbody:LExpr LMonoTy IDMeta),
-    σ.config.factory.getFactoryLFunc func_id.name = .some fn →
-    fn.body = .some fnbody →
-    Step σ (.op func_id _) fnbody
-
+-- A free variable. Stuck if fvar does not exist in LState.
 | expand_fvar:
   ∀ (σ:LState IDMeta) (x:Identifier IDMeta) (e:LExpr LMonoTy IDMeta),
-    σ.state.find? x = .some (_,e) →
-    Step σ (.fvar x _) e
+    σ.state.find? x = .some (ty,e) →
+    Step σ (.fvar x ty') e
 
 -- Beta reduction for lambda; Call-by-value semantics.
 | beta:
   ∀ (σ:LState IDMeta) (e1 v2:LExpr LMonoTy IDMeta),
     LExpr.isCanonicalValue σ v2 →
-    Step σ (.app (.abs _ e1) v2) (LExpr.subst e1 v2)
-
-| cbv:
-  ∀ (σ:LState IDMeta) (e1 e2 e2':LExpr LMonoTy IDMeta),
-    Step σ e2 e2' →
-    Step σ (.app e1 e2) (.app e1 e2')
+    Step σ (.app (.abs ty e1) v2) (LExpr.subst v2 e1)
 
 -- Universal quantification.
 | beta_univ:
-  ∀ (σ:LState IDMeta) (e1 v2:LExpr LMonoTy IDMeta),
+  ∀ (σ:LState IDMeta) (e1 v2 trig:LExpr LMonoTy IDMeta),
     LExpr.isCanonicalValue σ v2 →
-    Step σ (.app (.quant .all _ _ e1) v2) (LExpr.subst e1 v2)
+    Step σ (.app (.quant .all ty trig e1) v2) (LExpr.subst v2 e1)
+
+-- Call-by-value semantics.
+| reduce_2:
+  ∀ (σ:LState IDMeta) (v1 e2 e2':LExpr LMonoTy IDMeta),
+    LExpr.isCanonicalValue σ v1 →
+    Step σ e2 e2' →
+    Step σ (.app v1 e2) (.app v1 e2')
+
+| reduce_1:
+  ∀ (σ:LState IDMeta) (e1 e1' e2:LExpr LMonoTy IDMeta),
+    Step σ e1 e1' →
+    Step σ (.app e1 e2) (.app e1' e2)
 
 -- For ite x e1 e2, do not eagerly evaluate e1 and e2.
--- It is interpreted as 'ite x (λ.e1) (λ.e2)'.
-| beta_ite_then:
-  ∀ (σ:LState IDMeta) (econd ethen eelse:LExpr LMonoTy IDMeta),
-    econd = .const (.boolConst true) →
-    Step σ (.ite econd ethen eelse) ethen
+-- For the reduction order, ite x e1 e2 is interpreted as
+-- 'ite x (λ.e1) (λ.e2)'.
+| ite_beta_then:
+  ∀ (σ:LState IDMeta) (ethen eelse:LExpr LMonoTy IDMeta),
+    Step σ (.ite (.const (.boolConst true)) ethen eelse) ethen
 
-| beta_ite_else:
-  ∀ (σ:LState IDMeta) (econd ethen eelse:LExpr LMonoTy IDMeta),
-    econd = .const (.boolConst false) →
-    Step σ (.ite econd ethen eelse) eelse
+| ite_beta_else:
+  ∀ (σ:LState IDMeta) (ethen eelse:LExpr LMonoTy IDMeta),
+    Step σ (.ite (.const (.boolConst false)) ethen eelse) eelse
 
-| cbv_ite_cond:
+| ite_reduce_cond:
   ∀ (σ:LState IDMeta) (econd econd' ethen eelse:LExpr LMonoTy IDMeta),
     Step σ econd econd' →
     Step σ (.ite econd ethen eelse) (.ite econd' ethen eelse)
 
 -- Equality. Reduce after both operands evaluate to values.
-| beta_eq_true:
-  ∀ (σ:LState IDMeta) (e1 e2:LExpr LMonoTy IDMeta),
-    LExpr.isCanonicalValue σ e1 → LExpr.isCanonicalValue σ e2 →
-    e1 = e2 →
-    Step σ (.eq e1 e2) (.const (.boolConst true))
+| beta_eq:
+  ∀ (σ:LState IDMeta) (e1 e2:LExpr LMonoTy IDMeta)
+    (H1:LExpr.isCanonicalValue σ e1)
+    (H2:LExpr.isCanonicalValue σ e2),
+    Step σ (.eq e1 e2) (.const (.boolConst (LExpr.eql σ e1 e2 H1 H2)))
 
-| beta_eq_false:
-  ∀ (σ:LState IDMeta) (e1 e2:LExpr LMonoTy IDMeta),
-    LExpr.isCanonicalValue σ e1 → LExpr.isCanonicalValue σ e2 →
-    ¬ (e1 = e2) →
-    Step σ (.eq e1 e2) (.const (.boolConst false))
-
-| cbv_eq_lhs:
+| reduce_eq_lhs:
   ∀ (σ:LState IDMeta) (e1 e1' e2:LExpr LMonoTy IDMeta),
     Step σ e1 e1' →
     Step σ (.eq e1 e2) (.eq e1' e2)
 
-| cbv_eq_rhs:
-  ∀ (σ:LState IDMeta) (e1 e2 e2':LExpr LMonoTy IDMeta),
-    LExpr.isCanonicalValue σ e1 → Step σ e2 e2' →
-    Step σ (.eq e1 e2) (.eq e1 e2')
+| reduce_eq_rhs:
+  ∀ (σ:LState IDMeta) (v1 e2 e2':LExpr LMonoTy IDMeta),
+    LExpr.isCanonicalValue σ v1 → Step σ e2 e2' →
+    Step σ (.eq v1 e2) (.eq v1 e2')
 
 -- Evaluation keeps the metadata.
 | mdata:
@@ -102,4 +98,40 @@ inductive Step
     Step σ e e' →
     Step σ (.mdata m e) (.mdata m e')
 
-end Lamda
+-- Expand functions and free variables when they are evaluated.
+-- If the function body is unknown, concreteEval can be instead used. Look at
+-- the eval_fn constructor below.
+-- This is consistent with what LExpr.eval does (modulo the "inline" flag).
+| expand_fn:
+  ∀ (σ:LState IDMeta) (e callee fnbody new_body:LExpr LMonoTy IDMeta) args fn,
+    σ.config.factory.callOfLFunc e = .some (callee,args,fn) →
+    args.all (LExpr.isCanonicalValue σ) →
+    fn.body = .some fnbody →
+    new_body = LExpr.substFvars fnbody (fn.inputs.keys.zip args) →
+    Step σ e new_body
+
+-- The second way of evaluating a function call.
+-- If LFunc has a concrete evaluator, this can be used to 'jump' to the final
+-- result of the function.
+| eval_fn:
+  ∀ (σ:LState IDMeta) (e callee:LExpr LMonoTy IDMeta) args fn denotefn,
+    σ.config.factory.callOfLFunc e = .some (callee,args,fn) →
+    args.all (LExpr.isCanonicalValue σ) →
+    fn.concreteEval = .some denotefn →
+    Step σ e (denotefn (LExpr.mkApp callee args) args)
+
+
+theorem step_const_stuck:
+  ∀ (σ:LState IDMeta) x e, ¬ Step σ (.const x) e := by
+  intros σ x e H
+  contradiction
+
+/--
+Multi-step execution: reflexive transitive closure of single steps.
+-/
+inductive StepStar
+  : LState IDMeta → LExpr LMonoTy IDMeta → LExpr LMonoTy IDMeta → Prop where
+| refl : ∀ σ e, StepStar σ e e
+| step : ∀ σ e e' e'', Step σ e e' → StepStar σ e' e'' → StepStar σ e e''
+
+end Lambda
