StrataTest/DL/Lambda/LExprEvalTests.lean
@@ -4,6 +4,7 @@
   SPDX-License-Identifier: Apache-2.0 OR MIT
 -/
 
+import Strata.DL.Lambda.Semantics
 import Strata.DL.Lambda.LExprEval
 
 ---------------------------------------------------------------------
@@ -19,6 +20,12 @@ section EvalTest
 open LTy.Syntax LExpr.SyntaxMono
 open Std (ToFormat Format format)
 
+/-
+Each test is a pair of
+1. Lambda.LExpr.eval invocation, and
+2. Its equivalent Lambda.LExpr.Step version.
+-/
+
 /-- info: (λ (if (%0 == #1) then #10 else (_minit %0))) -/
 #guard_msgs in
 #eval format $ Lambda.LExpr.eval 100
@@ -26,15 +33,53 @@ open Std (ToFormat Format format)
                       [[("m", (mty[int → int], esM[_minit]))]] }
         esM[λ (if (%0 == #1) then #10 else (m %0))]
 
+-- Small step stucks because abstraction is a value.
+example:
+  ∀ σ e, ¬ (Lambda.Step σ (esM[(λ (if (%0 == #1) then #10 else (m %0)))]) e)
+  := by
+  intros σ e H
+  contradiction
+
+
 /-- info: #42 -/
 #guard_msgs in
 #eval format $ LExpr.eval 100
                           { LState.init with state := [[("x", (mty[int], esM[#32]))]] }
                           esM[((λ (if (%0 == #23) then #17 else #42)) (x : int))]
 
+example:
+  Lambda.StepStar
+    { LState.init with state := [[("x", (mty[int], esM[#32]))]] }
+    esM[((λ (if (%0 == #23) then #17 else #42)) (x : int))]
+    esM[#42] := by
+  apply StepStar.step
+  · apply Step.reduce_2
+    · unfold LExpr.isCanonicalValue; rfl
+    · repeat constructor
+  apply StepStar.step
+  · apply Step.beta; unfold isCanonicalValue; rfl
+  conv => lhs; reduce
+  apply StepStar.step
+  · apply Step.ite_reduce_cond
+    apply Step.beta_eq <;> unfold isCanonicalValue <;> rfl
+  conv => lhs; reduce
+  apply StepStar.step
+  · apply Step.ite_beta_else
+  apply StepStar.refl
+
+
 /-- info: (f #true) -/
 #guard_msgs in
 #eval format $ LExpr.eval 10 ∅ esM[(f #true)]
+
+theorem nil_state_empty {Ty}: (∅:LState Ty).state = [] := by
+  rfl
+
+example:
+  ∀ e, ¬ Lambda.Step ∅ esM[(f #true)] e := by
+  intros e H
+  contradiction
+
 
 /-- info: (minit #24) -/
 #guard_msgs in
@@ -44,24 +89,91 @@ open Std (ToFormat Format format)
                          [("m", (none, (.intConst 12)))]] }
                     esM[((λ (if (%0 == #23) then #17 else (m %0)) #24))]
 
+example:
+  Lambda.StepStar
+    { LState.init with state :=
+      [[("m", (none, esM[(λ (minit %0))]))], -- most recent scope
+      [("m", (none, (.intConst 12)))]] }
+    esM[((λ (if (%0 == #23) then #17 else (m %0)) #24))]
+    esM[(minit #24)] := by
+  apply StepStar.step
+  · apply Step.beta; unfold isCanonicalValue; rfl
+  conv => lhs; reduce
+  apply StepStar.step
+  · apply Step.ite_reduce_cond
+    apply Step.beta_eq <;> unfold isCanonicalValue <;> rfl
+  conv => lhs; reduce
+  apply StepStar.step
+  · apply Step.ite_beta_else
+  apply StepStar.step
+  · apply Step.reduce_1
+    apply Step.expand_fvar
+    rfl
+  apply StepStar.step
+  · apply Step.beta
+    unfold isCanonicalValue; rfl
+  apply StepStar.refl
+
+
 /-- info: (minit #24) -/
 #guard_msgs in
 #eval format $ LExpr.eval 100
                     { LState.init with state := [[("m", (none, esM[minit]))]] }
                     esM[((λ (if (%0 == #23) then #17 else (m %0))) #24)]
 
+example:
+  Lambda.StepStar
+    { LState.init with state := [[("m", (none, esM[minit]))]] }
+    esM[((λ (if (%0 == #23) then #17 else (m %0))) #24)]
+    esM[(minit #24)] := by
+  apply StepStar.step
+  · apply Step.beta; unfold isCanonicalValue; rfl
+  conv => lhs; reduce
+  apply StepStar.step
+  · apply Step.ite_reduce_cond
+    apply Step.beta_eq <;> unfold isCanonicalValue <;> rfl
+  conv => lhs; reduce
+  apply StepStar.step
+  · apply Step.ite_beta_else
+  apply StepStar.step
+  · apply Step.reduce_1
+    apply Step.expand_fvar
+    rfl
+  apply StepStar.refl
+
+
 /-- info: x -/
 #guard_msgs in
 #eval format $ LExpr.eval 10 ∅ esM[if #true then x else y]
+
+example:
+  Lambda.StepStar ∅ esM[if #true then x else y] esM[x] := by
+  apply StepStar.step
+  · constructor
+  apply StepStar.refl
+
 
 -- Ill-formed `abs` is returned as-is in this Curry style...
 /-- info: (λ %1) -/
 #guard_msgs in
 #eval format $ LExpr.eval 10 ∅ esM[(λ %1)]
 
+example:
+  ∀ e, ¬ Lambda.Step ∅ esM[(λ %1)] e := by
+  intros e H
+  contradiction
+
+
 /-- info: ((λ %1) #true) -/
 #guard_msgs in
 #eval format $ LExpr.eval (IDMeta:=Unit) 10 ∅ (.app (.mdata ⟨"x"⟩ (.abs .none (.bvar 1))) .true)
+
+example:
+  ∀ e, ¬ Lambda.Step (IDMeta:=Unit) ∅
+      (.app (.mdata ⟨"x"⟩ (.abs .none (.bvar 1))) .true) e := by
+  intros e H
+  contradiction
+
 
 /- Tests for evaluation of BuiltInFunctions. -/
 
@@ -119,29 +231,164 @@ private def testState : LState Unit :=
 #guard_msgs in
 #eval format $ LExpr.eval (IDMeta:=Unit) 10 testState esM[((~IntAddAlias #20) #30)]
 
+example:
+  Lambda.StepStar testState esM[((~IntAddAlias #20) #30)] esM[#50] := by
+  apply StepStar.step
+  · apply Step.expand_fn <;> try rfl
+    · simp only [HAppend.hAppend, Append.append, List.append, List.all]
+      unfold isCanonicalValue; rfl
+  apply StepStar.step
+  · apply Step.eval_fn
+    · rfl
+    · conv => lhs; reduce; unfold isCanonicalValue; reduce
+    · conv => lhs; rhs; reduce
+  apply StepStar.refl
+
 /-- info: ((~Int.Add #20) x) -/
 #guard_msgs in
 #eval format $ LExpr.eval (IDMeta:=Unit) 10 testState esM[((~IntAddAlias #20) x)]
 
+-- Note: this case diverges from concrete evaluator, because 'x' is not a
+-- canonical value! Small step reduces only when the arguments are values,
+-- to avoid nondeterminism in the small-step semantics (unless this becomes
+-- explicitly allowed in the future).
+example:
+  ∀ e, ¬ Lambda.Step testState esM[((~IntAddAlias #20) x)] e
+  := by
+  intro e H; cases H
+  case reduce_2 =>
+    contradiction
+  case reduce_1 =>
+    contradiction
+  case expand_fn =>
+    rename_i Hlfunc Hfv
+    conv at Hlfunc =>
+      lhs; reduce
+    cases Hlfunc
+    rename_i Hconst Htmp
+    conv at Hconst =>
+      lhs; reduce; unfold isCanonicalValue; reduce
+    contradiction
+  case eval_fn =>
+    rename_i Hlfunc
+    conv at Hlfunc =>
+      lhs; reduce
+    cases Hlfunc
+    rename_i Hconst Htmp
+    conv at Hconst =>
+      lhs; reduce; unfold isCanonicalValue; reduce
+    contradiction
+
+
+-- A sanity check that confirms the parse tree of λλ x y
+/-- info: true -/
+#guard_msgs in
+#eval esM[(λλ (~Int.Add %1) %0)] = esM[((λ(λ (~Int.Add %1))) %0)]
+
 /-- info: ((~Int.Add ((~Int.Add #5) #100)) x) -/
 #guard_msgs in
-#eval format $ LExpr.eval (IDMeta:=Unit) 10 LState.init esM[(( ((λλ (~Int.Add %1) %0)) ((λ ((~Int.Add %0) #100)) #5)) x)]
+#eval format $ LExpr.eval (IDMeta:=Unit) 10 LState.init
+  esM[(( ((λ(λ ((~Int.Add %1) %0)))) ((λ ((~Int.Add %0) #100)) #5)) x)]
+
+-- The small step semantics of this example will stuck in the middle because
+-- 'Int.Add %0 100' cannot be evaluated because the definition of Int.Add is
+-- not available in LState.init .
+
 
 /-- info: #50 -/
 #guard_msgs in
 #eval format $ LExpr.eval (IDMeta:=Unit) 10 testState esM[((~Int.Add #20) #30)]
 
+example:
+  Lambda.StepStar testState esM[((~Int.Add #20) #30)] esM[#50] := by
+  apply StepStar.step
+  · apply Step.eval_fn <;> try rfl
+    · conv => lhs; reduce; unfold isCanonicalValue; reduce
+  apply StepStar.refl
+
+
 /-- info: ((~Int.Add #105) x) -/
 #guard_msgs in
-#eval format $ LExpr.eval (IDMeta:=Unit) 10 testState esM[((((λλ (~Int.Add %1) %0)) ((λ ((~Int.Add %0) #100)) #5)) x)]
+#eval format $ LExpr.eval (IDMeta:=Unit) 10 testState
+  esM[((((λ(λ (~Int.Add %1) %0))) ((λ ((~Int.Add %0) #100)) #5)) x)]
+
+/-- info: false -/
+#guard_msgs in
+#eval LExpr.isCanonicalValue testState esM[((~Int.Add #100) #200)]
+
+/-- info: true -/
+#guard_msgs in
+#eval LExpr.isCanonicalValue testState esM[(~Int.Add #100)]
+
+example:
+  Lambda.StepStar testState
+    esM[((((λ(λ (~Int.Add %1) %0))) ((λ ((~Int.Add %0) #100)) #5)) x)]
+    esM[((~Int.Add #105) x)] := by
+  unfold LExpr.absUntyped
+  apply StepStar.step
+  · apply Step.reduce_1
+    apply Step.reduce_2
+    · unfold isCanonicalValue; rfl
+    · apply Step.beta
+      · unfold isCanonicalValue; rfl
+  conv => lhs; reduce
+  apply StepStar.step
+  · apply Step.reduce_1
+    apply Step.reduce_2
+    · unfold isCanonicalValue; rfl
+    · apply Step.eval_fn
+      · conv => lhs; reduce; unfold isCanonicalValue; reduce
+      · conv => lhs; reduce; unfold isCanonicalValue; reduce
+      · conv => lhs; reduce
+  conv => lhs; reduce
+  apply StepStar.step
+  · apply Step.reduce_1
+    apply Step.beta
+    · unfold isCanonicalValue; rfl
+  conv => lhs; reduce
+  apply StepStar.step
+  · apply Step.reduce_1
+    apply Step.beta
+    · unfold isCanonicalValue; rfl
+  conv => lhs; reduce
+  apply StepStar.refl
+
 
 /-- info: ((#f #20) #-5) -/
 #guard_msgs in
-#eval format $ LExpr.eval (IDMeta:=Unit) 10 testState esM[( ((λλ (#f %1) %0) #20) ((λ (~Int.Neg %0)) #5))]
+#eval format $ LExpr.eval (IDMeta:=Unit) 10 testState
+  esM[( ((λ(λ (#f %1) %0) #20)) ((λ (~Int.Neg %0)) #5))]
+
+-- The small step semantics of this example will stuck in the middle because
+-- '(#f 20) e' cannot be evaluated because the definition of #f is
+-- not available.
+
 
 /-- info: ((~Int.Add #20) (~Int.Neg x)) -/
 #guard_msgs in
-#eval format $ LExpr.eval (IDMeta:=Unit) 10 testState esM[( ((λλ (~Int.Add %1) %0) #20) ((λ (~Int.Neg %0)) x))]
+#eval format $ LExpr.eval (IDMeta:=Unit) 10 testState
+  esM[( ((λ(λ (~Int.Add %1) %0)) #20) ((λ (~Int.Neg %0)) x))]
+
+-- The result stops at (.. ((λ (~Int.Neg %0)) x)) because definition of
+-- x is not available.
+example:
+  Lambda.StepStar testState
+    esM[( ((λ(λ (~Int.Add %1) %0)) #20) ((λ (~Int.Neg %0)) x))]
+    esM[((~Int.Add #20) ((λ (~Int.Neg %0)) x))]
+  := by
+  unfold LExpr.absUntyped
+  apply StepStar.step
+  · apply Step.reduce_1
+    apply Step.beta
+    · conv => lhs; reduce; unfold isCanonicalValue; reduce
+  conv => lhs; reduce
+  apply StepStar.step
+  · apply Step.reduce_1
+    apply Step.beta
+    · conv => lhs; reduce; unfold isCanonicalValue; reduce
+  conv => lhs; reduce
+  apply StepStar.refl
+
 
 /-- info: ((~Int.Add #20) (~Int.Neg x)) -/
 #guard_msgs in
@@ -155,21 +402,106 @@ private def testState : LState Unit :=
 #guard_msgs in
 #eval format $ LExpr.eval (IDMeta:=Unit) 10 testState esM[((λ %0) ((~Int.Add #20) #30))]
 
+example:
+  Lambda.StepStar testState
+    esM[((λ %0) ((~Int.Add #20) #30))]
+    esM[(#50)]
+  := by
+  unfold LExpr.absUntyped
+  apply StepStar.step
+  · apply Step.reduce_2
+    · conv => lhs; reduce; unfold isCanonicalValue; reduce
+    · apply Step.eval_fn <;> try rfl
+      · conv => lhs; reduce; unfold isCanonicalValue; reduce
+  conv => lhs; reduce
+  apply StepStar.step
+  · apply Step.beta
+    · conv => lhs; reduce; unfold isCanonicalValue; reduce
+  conv => lhs; reduce
+  apply StepStar.refl
+
+
 /-- info: #100 -/
 #guard_msgs in
 #eval format $ LExpr.eval (IDMeta:=Unit) 10 testState esM[((~Int.Div #300) ((~Int.Add #2) #1))]
+
+example:
+  Lambda.StepStar testState esM[((~Int.Div #300) ((~Int.Add #2) #1))] esM[(#100)]
+  := by
+  apply StepStar.step
+  · apply Step.reduce_2
+    · conv => lhs; reduce; unfold isCanonicalValue; reduce; unfold isCanonicalValue
+    · apply Step.eval_fn <;> try rfl
+      · conv => lhs; reduce; unfold isCanonicalValue; reduce
+  conv => lhs; reduce
+  apply StepStar.step
+  · apply Step.eval_fn <;> try rfl
+    · conv => lhs; reduce; unfold isCanonicalValue; reduce
+  conv => lhs; reduce
+  apply StepStar.refl
 
 /-- info: #0 -/
 #guard_msgs in
 #eval format $ LExpr.eval (IDMeta:=Unit) 10 testState esM[((~Int.Add #3) (~Int.Neg #3))]
 
+example:
+  Lambda.StepStar testState esM[((~Int.Add #3) (~Int.Neg #3))] esM[(#0)]
+  := by
+  apply StepStar.step
+  · apply Step.reduce_2
+    · conv => lhs; reduce; unfold isCanonicalValue; reduce; unfold isCanonicalValue
+    · apply Step.eval_fn <;> try rfl
+      · conv => lhs; reduce; unfold isCanonicalValue; reduce
+  conv => lhs; reduce
+  apply StepStar.step
+  · apply Step.eval_fn <;> try rfl
+    · conv => lhs; reduce; unfold isCanonicalValue; reduce
+  conv => lhs; reduce
+  apply StepStar.refl
+
 /-- info: #0 -/
 #guard_msgs in
 #eval format $ LExpr.eval (IDMeta:=Unit) 10 testState esM[((~Int.Add (~Int.Neg #3)) #3)]
 
+example:
+  Lambda.StepStar testState esM[((~Int.Add (~Int.Neg #3)) #3)] esM[(#0)]
+  := by
+  apply StepStar.step
+  · apply Step.reduce_1
+    apply Step.reduce_2
+    · conv => lhs; reduce; unfold isCanonicalValue; reduce; unfold isCanonicalValue
+    · apply Step.eval_fn <;> try rfl
+      · conv => lhs; reduce; unfold isCanonicalValue; reduce; unfold isCanonicalValue
+  conv => lhs; reduce
+  apply StepStar.step
+  · apply Step.eval_fn <;> try rfl
+    · conv => lhs; reduce; unfold isCanonicalValue; reduce; unfold isCanonicalValue
+  apply StepStar.refl
+
 /-- info: ((~Int.Div #300) #0) -/
 #guard_msgs in
 #eval format $ LExpr.eval (IDMeta:=Unit) 10 testState esM[((~Int.Div #300) ((~Int.Add #3) (~Int.Neg #3)))]
+
+example:
+  Lambda.StepStar testState
+    esM[((~Int.Div #300) ((~Int.Add #3) (~Int.Neg #3)))]
+    esM[((~Int.Div #300) #0)]
+  := by
+  apply StepStar.step
+  · apply Step.reduce_2
+    · conv => lhs; reduce; unfold isCanonicalValue; reduce; unfold isCanonicalValue
+    · apply Step.reduce_2
+      · conv => lhs; reduce; unfold isCanonicalValue; reduce; unfold isCanonicalValue
+      · apply Step.eval_fn <;> try rfl
+        · conv => lhs; reduce; unfold isCanonicalValue; reduce; unfold isCanonicalValue
+  conv => lhs; reduce
+  apply StepStar.step
+  · apply Step.reduce_2
+    · conv => lhs; reduce; unfold isCanonicalValue; reduce; unfold isCanonicalValue
+    · apply Step.eval_fn <;> try rfl
+      · conv => lhs; reduce; unfold isCanonicalValue; reduce; unfold isCanonicalValue
+  conv => lhs; reduce
+  apply StepStar.refl
 
 /-- info: ((~Int.Div x) #3) -/
 #guard_msgs in
